tmp

theories/instantiation_properties.v
@@ -30,6 +30,326 @@ Variable executable_host_instance : executable_host.
 Let host_event := host_event executable_host_instance.
 
 Let instantiate := instantiate host_function host_instance.
+Let instantiate_simpl := instantiate_simpl host_function.
+(*
+Let tab_agree := @typing.tab_agree host_function.
+*)
+Inductive ext_typing_list: store_record -> seq module_export -> seq extern_t -> Prop :=
+| ext_typing_list_nil: forall s,
+    ext_typing_list s [::] [::]
+| ext_typing_list_cons: forall s v_exp v_exps te tes,
+    ext_typing_list s v_exps tes ->
+    external_typing s (modexp_desc v_exp) te ->
+    ext_typing_list s (v_exp :: v_exps) (te :: tes).
+
+
+Lemma instantiation_sound (s: store_record) m v_imps s' inst v_exps start:
+  store_typing s ->
+  instantiate s m v_imps ((s', inst, v_exps), start) ->
+  (store_typing s') /\
+  (exists C, inst_typing s' inst C) /\
+  (exists tes, ext_typing_list s' v_exps tes) /\
+  (pred_option (fun i => i < length s'.(s_funcs)) start).
+  (* /\ store_extension s s' *)
+Proof.
+Admitted.
+
+Let tab_agree := @tab_agree host_function.
+
+Lemma tab_agree_aux s_funcs s_tables s_mems s_globals tab func:
+  tab_agree {| s_funcs := s_funcs; s_tables := s_tables; s_mems := s_mems; s_globals := s_globals |} tab ->
+  tab_agree {| s_funcs := List.app s_funcs [:: func]; s_tables := s_tables; s_mems := s_mems;
+               s_globals := s_globals |} tab .
+Proof.
+  rewrite /tab_agree /typing.tab_agree.
+  move => Htb.
+  destruct Htb as [Htable Hs_tables]; subst.
+  constructor.
+  - (* forall tabcl_agree (table_data tab) *)
+    induction (table_data tab) as [| hd tl IH]; first by constructor.
+    (* forall tabcl_agree hd :: tl *)
+    inversion Htable as [| x y Hhd Htl]; subst.
+    constructor.
+    (* tabcl_agree hd *)
+    destruct hd => //=. 
+    rewrite /tabcl_agree in Hhd. simpl in Hhd.
+    rewrite size_cat. by rewrite ltn_addr.
+    (* forall tabcl_agree tl *)
+    apply IH. exact Htl.
+  - (* tabsize_agree table *)
+    assumption.
+Qed.
+
+Let functions_agree := @functions_agree host_function.
+
+Lemma functions_agree_aux s_funcs func f tf: 
+  functions_agree s_funcs f tf ->
+  functions_agree (List.app s_funcs [:: func]) f tf.
+Proof.
+  rewrite /functions_agree /typing.functions_agree.
+  move/andP => [H1 H2]. move/eqP in H2.
+  apply/andP. split.
+  + (* f < length (s_funcs [::func])  *)
+    rewrite List.app_length.
+    by rewrite ltn_addr.
+  + (* option_map cl_type (List.nth_error (s_funcs [::func]) f) == Some tf *)
+    apply/eqP.
+    rewrite <-H2.
+    apply f_equal.
+    apply List.nth_error_app1.
+    by apply/ltP.
+Qed.
+
+
+Lemma all2_forward: forall A B (f1 f2 : A -> B -> bool) l1 l2,
+  (forall a b, f1 a b -> f2 a b) ->
+  (all2 f1 l1 l2 -> all2 f2 l1 l2).
+Proof.
+  move=> A B f1 f2. elim.
+  - by case.
+  - move=> h1 l1 IH. case=> //= h2 l2 E.
+    move/andP => [H1 H2].
+    apply/andP. split.
+    + by apply E.
+    + by apply IH => //=.
+Qed.
+
+Let cl_type_check_single := @cl_type_check_single host_function.
+
+Lemma cl_type_check_single_aux1 s_funcs s_tables s_mems s_globals inst m_f func:
+  cl_type_check_single {| s_funcs := s_funcs; s_tables := s_tables; s_mems := s_mems; s_globals := s_globals |} func ->
+  cl_type_check_single {| s_funcs := s_funcs ++ 
+                                     [:: FC_func_native inst
+                                         (List.nth match modfunc_type m_f with
+                                            | Mk_typeidx n => n
+                                            end (inst_types inst) (Tf [::] [::])) (modfunc_locals m_f) 
+                                         (modfunc_body m_f)]; 
+                          s_tables := s_tables; s_mems := s_mems; s_globals := s_globals |} func.
+Proof.
+  move => Hcl.
+  destruct Hcl as [tf' Hcl_typing].
+  exists tf'.
+  destruct func as [i tf ts es | tf h].
+  + (* cl_typing_native *)
+    inversion Hcl_typing; subst.
+    rename H4 into Hinst_typing. rename H8 into Hbe_typing.
+    apply cl_typing_native
+      with (C := C)
+           (C' := upd_local_label_return C (tc_local C ++ t1s ++ ts) ([::t2s] ++ tc_label C) (Some t2s))
+          => //=.
+    destruct C.
+    rewrite /inst_typing. simpl.
+    rewrite /inst_typing in Hinst_typing. simpl in Hinst_typing.
+    destruct tc_local => //=.
+    destruct tc_label => //=.
+    destruct tc_return => //=.
+    destruct i.
+    move/andP in Hinst_typing. destruct Hinst_typing as [Hinst_typing Hmem].
+    move/andP in Hinst_typing. destruct Hinst_typing as [Hinst_typing Htab].
+    move/andP in Hinst_typing. destruct Hinst_typing as [Hinst_typing Hglb].
+    move/andP in Hinst_typing. destruct Hinst_typing as [Hty Hfunc].
+    move/eqP in Hty; subst.
+    apply/andP. split => //=.
+    apply/andP. split => //=.
+    apply/andP. split => //=.
+    apply/andP. split => //=.
+    eapply all2_forward.
+    apply functions_agree_aux.
+    by exact Hfunc.
+  + (* cl_typing_host *)
+    inversion Hcl_typing; subst.
+    by apply cl_typing_host.
+Qed.
+
+Axiom Forall_app
+     : forall (A : Type) (P : A -> Prop) (l1 l2 : seq A),
+       List.Forall P (l1 ++ l2)%list <-> List.Forall P l1 /\ List.Forall P l2.
+
+Lemma store_typing_preserve_add_func : forall s_funcs s_tables s_mems s_globals inst m_f,
+    store_typing
+      {| s_funcs := s_funcs; s_tables := s_tables; s_mems := s_mems; s_globals := s_globals |} ->
+    (*
+    module_func_typing 
+    add_func s _ _ ...
+*)
+    store_typing
+      {| s_funcs :=
+        List.app s_funcs
+                 [:: FC_func_native
+                     inst
+                     (List.nth (match m_f.(modfunc_type) with | Mk_typeidx n => n end) inst.(inst_types) (Tf nil nil))
+                     m_f.(modfunc_locals)
+                     m_f.(modfunc_body)]
+      ; s_tables := s_tables; s_mems := s_mems; s_globals := s_globals |}.
+Proof.
+  move=> s_funcs s_tables s_mems s_globals inst m_f HSTyping.
+  Print store_typing.
+  inversion HSTyping as [Hcl [ Htb Hmem ]].
+  constructor.
+  - (* cl_typing *)
+    rewrite Forall_app.
+    split.
+    + (* forall cl_type_check_single s_funcs *) 
+      apply List.Forall_forall => func Hin.
+      rewrite -> List.Forall_forall in Hcl.
+      apply cl_type_check_single_aux1.
+      by apply Hcl.
+    + (* cl_typing_check_single func *) {
+        constructor => //=.
+        remember (List.nth match modfunc_type m_f with
+                           | Mk_typeidx n => n
+                           end (inst_types inst) (Tf [::] [::])) as tf.
+        exists tf.
+        destruct tf as [t1s t2s]. Check List.map.  Search (N).
+        eapply cl_typing_native => //.
+        * admit.
+        * admit.
+          Admitted. (*
+        remember ({| tc_types_t := inst.(inst_types);
+                     tc_func_t := (List.map cl_type s_funcs) ++ [:: (Tf t1s t2s)];
+                     tc_global := List.map (fun g => Build_global_type (g_mut g) (typeof (g_val g))) s_globals;
+                     tc_table := List.map
+                                 (fun t => {| tt_limits := {| lim_min := N.of_nat(tab_size t);
+                                                              lim_max := Some (N.of_nat(t.(table_max_opt) + 1)) |};
+                                              tt_elem_type := ELT_funcref |})
+                                 s_tables;
+                     tc_memory := List.map
+                                  (fun m => {| lim_min := (mem_size m); lim_max := m.(mem_max_opt) |})
+                                s_mems;
+                     tc_local := nil;
+                     tc_label := nil;
+                    tc_return := None |}) as C.
+        apply cl_typing_native with
+          (C := C)
+          (C' := upd_local_label_return C (tc_local C ++ t1s ++ (modfunc_locals m_f)) ([::t2s] ++ tc_label C) (Some t2s)) => //=.
+        * (* inst_typing *)
+          destruct inst. destruct C. simpl.
+          destruct tc_local => //=.
+          destruct tc_label => //=.
+          destruct tc_return => //=.
+          inversion HeqC; subst.
+          destruct HeqC. 
+          apply/andP. split.
+          apply/andP. split.
+          apply/andP. split.
+          apply/andP. split => //=.
+          -- (* functions_agree *) {
+            admit.
+          }
+          -- (* globals_agree *) {
+              rewrite /globals_agree.
+            }
+            
+      }
+  split.
+  - (* tab_agree *)
+    apply List.Forall_forall => tab Hin.
+    rewrite -> List.Forall_forall in Htb.
+    apply tab_agree_aux.
+    by apply Htb.
+  - (* mem_agree *)
+    assumption.
+Admitted.*)
+
+Print module_typing.
+
+Print alloc_Xs.
+
+Print module_typing.
+Print module_func_typing.
+
+Lemma instantiation_sound_aux s s0 m inst l t_imps t_exps:
+  module_typing m t_imps t_exps ->
+  store_typing s ->
+  (s0, l) = alloc_Xs host_function 
+            (fun s m_f => alloc_func host_function s m_f inst) s (mod_funcs m) ->
+  (*
+  (s0, l) =
+           (let
+            '(s', fas) :=
+             List.fold_left
+               (fun '(s, ys) (x : module_func)
+                  => let '(s', y) := alloc_func host_function s x inst in (s', y :: ys))
+               (mod_funcs m) (s, acc) in (s', List.rev fas)) ->*)
+  store_typing s0.
+Proof.
+  move => Hmodule.
+  unfold module_typing in Hmodule.
+  destruct Hmodule as [fts [gts Hmodule]].
+  destruct m.
+  destruct Hmodule as [Hmodfunc _].
+  generalize dependent s.
+  generalize dependent acc.
+  generalize dependent fts.
+  generalize dependent mod_funcs.
+  induction mod_funcs => //; move => fts Hmodfunc acc s HType H0.
+  - simpl in H0.
+    by inversion H0; subst.
+  - simpl in H0.
+    destruct fts as [|ft fts']; first by inversion Hmodfunc.
+    inversion Hmodfunc; subst; clear Hmodfunc.
+    apply IHmod_funcs with(fts := fts') in H0 => //.
+    + admit.
+    + unfold add_func. 
+      apply store_typing_preserve_add_func.
+      by destruct s => //.
+Admitted.
+  
+Lemma instantiation_sound_simpl:  forall (s: store_record) m v_imps s' inst v_exps start,
+  store_typing s ->
+  instantiate_simpl s m v_imps ((s', inst, v_exps), start) ->
+  (store_typing s').
+  (* (exists C, inst_typing s' inst C) /\
+  (exists tes, ext_typing_list s' v_exps tes) /\
+  (pred_option (fun i => i < length s'.(s_funcs)) start).*)
+  (* /\ store_extension s s' *)
+Proof.
+  move=> s m v_imps s' inst v_exps start HType HInst. inversion HInst as [t_imps [t_exps [Hmodule H0]]].
+  unfold alloc_funcs_bool in H0.
+  remember (alloc_funcs host_function s (mod_funcs m) inst) as psi.
+  destruct psi.
+  rewrite /alloc_funcs in Heqpsi. (*/alloc_Xs in Heqpsi.*)
+  move/andP in H0.
+  destruct H0 as [Heqs Heqinst].
+  move/eqP in Heqs; subst.
+  move/eqP in Heqinst.
+  apply instantiation_sound_aux in Heqpsi => //.
+Qed.
+
+
+
+From mathcomp Require Import ssreflect ssrbool ssrnat eqtype seq.
+From ITree Require Import ITree.
+From ITree Require ITreeFacts.
+From Wasm Require Import list_extra datatypes datatypes_properties
+                         interpreter binary_format_parser operations
+                         typing opsem type_checker memory memory_list instantiation.
+From Coq Require Import BinNat.
+
+Section Host.
+
+Variable host_function : eqType.
+Let host := host host_function.
+
+Variable host_instance : host.
+
+Let store_record_eq_dec := @store_record_eq_dec host_function.
+Let store_record_eqType := @store_record_eqType host_function.
+
+Local Canonical Structure name_eqType := Eval hnf in EqType name (seq_eqMixin _).
+
+Let store_record := store_record host_function.
+Let host_state := host_state host_instance.
+
+Let store_typing := @store_typing host_function.
+
+Let external_typing := @external_typing host_function.
+
+Let executable_host := executable_host host_function.
+Variable executable_host_instance : executable_host.
+Let host_event := host_event executable_host_instance.
+
+Let instantiate := instantiate host_function host_instance.
 
 
 Inductive ext_typing_list: store_record -> seq module_export -> seq extern_t -> Prop :=
